Examples/IMP/Analysis/Sign.lean
@@ -1,3 +1,1 @@
 import Examples.IMP.Analysis.Sign.Defs
-import Examples.IMP.Analysis.Sign.Lemmas
-import Examples.IMP.Analysis.Sign.Soundness
